attic/equations_blit.v
@@ -1,0 +1,65 @@
+(* -------------------------------------------------------------------------- *)
+
+(* From array.v: *)
+
+(* In order to allow a fair comparison, let's define a third naive [blit],
+   this time using Equations, but without a higher-order function. *)
+
+(* A micro-benchmark (benchmark.v) suggests that, when running inside Rocq
+   using [vm_compute], [equations_blit] can be 75 times slower than
+   [simple_blit]. *)
+
+Section Code.
+Open Scope uint63.
+
+Equations equations_blit a _i b _j _n : array A
+by wf _n ilt :=
+equations_blit a _i b _j _n :=
+  IF _n =? 0 THEN
+    b
+  ELSE
+    do x ← get a _i ;
+    do b ← set b _j x ;
+    equations_blit a (_i + 1) b (_j + 1) (_n - 1).
+
+End Code.
+
+(* [equations_blit] is correct. *)
+
+Lemma wp_equations_blit :
+  ∀Int _n n,
+  blit_spec (λ a _i b _j, equations_blit a _i b _j _n) n.
+Proof.
+  by well-founded induction on _n along ilt.
+  unfold blit_spec. intros. arrays.
+  autorewrite with equations_blit.
+  wp_if.
+  (* Base case. *)
+  { wp_ret. isArray. }
+  (* Step case. *)
+  { wp_get x.
+    wp_set.
+    wp_op IH shadowing: b.
+    isArray. }
+Qed.
+
+(* -------------------------------------------------------------------------- *)
+
+(* From benchmark.v: *)
+
+(* The times in comments use OCaml 4.14.2+flambda. *)
+
+Time Definition a : array int :=
+  Eval vm_compute in
+  init n data.
+    (* 0.05 seconds : 1 million elements/second *)
+
+Time Definition b : array int :=
+  Eval vm_compute in
+  init n data.
+    (* same as [a] *)
+
+Time Definition time_equations_blit :=
+  Eval vm_compute in
+  (equations_blit a 0 b 0 n)%uint63.
+    (* 4.7 seconds : 10,500 elements/second *)
