src/benchmark.v
@@ -50,16 +50,6 @@ Time Definition time_simple_blit :=
   (simple_blit a 0 b' 0 n)%uint63.
     (* 0.06 seconds : 830,000 elements/second *)
 
-Time Definition b'' : array int :=
-  Eval vm_compute in
-  init n data.
-    (* same as [a] *)
-
-Time Definition time_equations_blit :=
-  Eval vm_compute in
-  (equations_blit a 0 b'' 0 n)%uint63.
-    (* 4.7 seconds : 10,500 elements/second *)
-
 Time Definition b''' : array int :=
   Eval vm_compute in
   init n data.
